examples/delayed_echo/EchoMain.v
@@ -1,0 +1,62 @@
+Require Import Coqlib.
+Require Import Universe.
+Require Import STS.
+Require Import Behavior.
+Require Import ModSem.
+Require Import Skeleton.
+Require Import PCM.
+Require Import HoareDef.
+Require Import Echo1.
+Require Import TODOYJ.
+
+Generalizable Variables E R A B C X Y Σ.
+
+Set Implicit Arguments.
+
+
+
+Section PROOF.
+
+  Context `{Σ: GRA.t}.
+
+  Definition mainF: Any.t -> itree Es val :=
+    fun varg =>
+      ccall "echo" [Vnullptr];;
+
+
+      call
+      '(ll, nref) <- (pop2F_parg varg)?;;
+      `b: val <- (ccall "cmp"  [ll; Vnullptr]);;
+      if (is_zero b)
+      then (
+          '(blk, ofs) <- (unptr ll)?;;
+          let addr_val  := Vptr blk ofs in
+          let addr_next := Vptr blk (ofs + 1) in
+          `v: val    <- (ccall "load"  [addr_val]);;
+          `next: val <- (ccall "load"  [addr_next]);;
+          `_: val    <- (ccall "free"  [addr_val]);;
+          `_: val    <- (ccall "free"  [addr_next]);; (*** change "free"s specification ***)
+          `_: val    <- (ccall "store" [nref; v]);;
+          Ret next
+        )
+      else Ret Vnullptr
+  .
+
+
+  Definition mainF: Any.t -> itree Es Any.t :=
+    fun varg =>
+      r <- trigger (Call "f" [Vint 10]↑);;
+      Ret r.
+
+  Definition mainSem: ModSem.t := {|
+    ModSem.fnsems := [("main", mainF)];
+    ModSem.initial_mrs := [("Main", (ε, tt↑))];
+  |}
+  .
+
+  Definition main: Mod.t := {|
+    Mod.get_modsem := fun _ => mainSem;
+    Mod.sk := [("Main", Sk.Gfun)];
+  |}
+  .
+End PROOF.
